Add Callstate in Sem.v && add sm_init in SimModSem, compiles AdqLocal

proof/AdequacyLocal.v
@@ -449,7 +449,7 @@ Section ADQMATCH.
   (* Simulation can go continuation when SimMem.t bigger than argument is given, (after unlifting it) *)
   (* with after_external fed with regsets sent. *)
   Inductive lxsim_stack: regset -> regset -> SimMem.t ->
-                         sem_src.(Smallstep.state) -> sem_tgt.(Smallstep.state) -> Prop :=
+                         list Frame.t -> list Frame.t -> Prop :=
   | lxsim_stack_nil
       rs_init_src rs_init_tgt sm0
     :
@@ -465,6 +465,8 @@ Section ADQMATCH.
       (MWF: SimMem.wf sm_arg)
       (GE: sim_ge sm_arg sem_src.(globalenv) sem_tgt.(globalenv))
       (MLE: SimMem.le tail_sm sm_arg)
+      sm_init
+      (MLE: SimMem.le (SimMem.lift sm_arg) sm_init)
       (K: forall
           sm_ret rs_ret_src rs_ret_tgt
           (MEMLE: SimMem.le (SimMem.lift sm_arg) sm_ret)
@@ -499,11 +501,26 @@ Section ADQMATCH.
                                                   lst_tgt1>>)>>))
     :
       lxsim_stack rs_arg_src rs_arg_tgt
-                  (SimMem.lift sm_arg)
+                  sm_init
                   ((Frame.mk ms_src rs_init_src lst_src0) :: tail_src)
                   ((Frame.mk ms_tgt rs_init_tgt lst_tgt0) :: tail_tgt)
 
   .
+
+  Lemma lxsim_stack_le
+        rs_init_src rs_init_tgt sm0 frs_src frs_tgt
+        (SIMSTACK: lxsim_stack rs_init_src rs_init_tgt sm0 frs_src frs_tgt)
+        sm1
+        (MLE: SimMem.le sm0 sm1)
+    :
+      <<SIMSTACK: lxsim_stack rs_init_src rs_init_tgt sm1 frs_src frs_tgt>>
+  .
+  Proof.
+    inv SIMSTACK.
+    { econs 1; eauto. }
+    econs 2; eauto.
+    etransitivity; eauto.
+  Qed.
 
   Inductive lxsim_lift: idx -> sem_src.(Smallstep.state) -> sem_tgt.(Smallstep.state) -> SimMem.t -> Prop :=
   | lxsim_lift_intro
@@ -520,9 +537,23 @@ Section ADQMATCH.
                   i0 lst_src lst_tgt sm0)
     :
       lxsim_lift i0
-                 ((Frame.mk ms_src rs_init_src lst_src) :: tail_src)
-                 ((Frame.mk ms_tgt rs_init_tgt lst_tgt) :: tail_tgt)
+                 (State ((Frame.mk ms_src rs_init_src lst_src) :: tail_src))
+                 (State ((Frame.mk ms_tgt rs_init_tgt lst_tgt) :: tail_tgt))
                  sm0
+  | lxsim_lift_callstate
+       sm_arg
+       (GE: sim_ge sm_arg sem_src.(globalenv) sem_tgt.(globalenv))
+       tail_src tail_tgt tail_sm
+       rs_arg_src rs_arg_tgt
+       (STACK: lxsim_stack rs_arg_src rs_arg_tgt tail_sm tail_src tail_tgt)
+       (MLE: SimMem.le tail_sm sm_arg)
+       (MWF: SimMem.wf sm_arg)
+       (SIMRS: (SimMem.sim_regset) sm_arg rs_arg_src rs_arg_tgt)
+    :
+      lxsim_lift idx_bot
+                 (Callstate rs_arg_src sm_arg.(SimMem.src_mem) tail_src)
+                 (Callstate rs_arg_tgt sm_arg.(SimMem.tgt_mem) tail_tgt)
+                 sm_arg
   .
 
 End ADQMATCH.
@@ -555,112 +586,6 @@ Section ADQINIT.
   Let sem_tgt := Sem.semantics p_tgt.
   Print Sem.initial_state.
 
-  Theorem init_lxsim_lift_progress
-          st_init_src
-          (INITSRC: sem_src.(Smallstep.initial_state) st_init_src)
-    :
-      exists st_init_tgt,
-        <<INITTGT: sem_tgt.(Smallstep.initial_state) st_init_tgt>>
-  .
-  Proof.
-    inv INITSRC; ss.
-    rename sk_link into sk_link_src.
-    rename st_init into st_init_src.
-    rename ms into ms_src. rename m into m_src.
-    rename INIT into INITSRC. rename INITSK into INITSKSRC. rename INITMEM into INITMEMSRC.
-    (* inv MSFIND. *)
-    (* rename blk into blk_src. rename if_sig into if_sig_src. rename FPTR into FPTRSRC. *)
-    (* rename MODSEM into MODSEMSRC. rename INTERNAL into INTERNALSRC. *)
-
-    exploit sim_link_sk; eauto. i; des. fold p_tgt in LOADTGT.
-    exploit init_sim_ge_strong; eauto. i; des. clarify.
-    ss. des_ifs.
-
-    assert(SIMFPTR: SimMem.sim_val sm_init (Genv.symbol_address (Genv.globalenv sk_link_src)
-                                                                (prog_main sk_link_src) Ptrofs.zero)
-                                   (Genv.symbol_address (Genv.globalenv sk_link_tgt)
-                                                        (prog_main sk_link_tgt) Ptrofs.zero)).
-    { admit "strengthen sim_skenv specs". }
-
-    exploit find_fptr_owner_fsim; eauto. i; des. clarify.
-    inv SIMMS.
-    inv MSFIND. inv FINDTGT.
-    assert(SIMRS: SimMem.sim_regset sm_init
-        (init_regs (Genv.symbol_address (Sk.load_skenv sk_link_src) (prog_main sk_link_src) Ptrofs.zero))
-        (init_regs (Genv.symbol_address (Sk.load_skenv sk_link_tgt) (prog_main sk_link_tgt) Ptrofs.zero))).
-    { u. ii. ss.
-      unfold Pregmap.set.
-      des_ifs.
-      - admit "strengthen sim_val".
-      - admit "strengthen sim_val".
-      - admit "strengthen sim_val".
-    }
-    exploit SIM; eauto. i; des.
-    bar.
-    exploit INITPROGRESS; eauto. i; des.
-    esplits; eauto. econs; eauto. econs; eauto.
-  Qed.
-
-  Theorem init_lxsim_lift_backward
-          st_init_tgt
-          (INITTGT: sem_tgt.(Smallstep.initial_state) st_init_tgt)
-          (SAFESRC: __guard__ (exists _st_init_src, sem_src.(Smallstep.initial_state) _st_init_src))
-    :
-      exists idx st_init_src sm_init,
-        <<INITTGT: sem_src.(Smallstep.initial_state) st_init_src>>
-        /\ <<SIM: lxsim_lift idx st_init_src st_init_tgt sm_init>>
-  .
-  Proof.
-    (* inv SAFESRC; ss. *)
-    (* rename sk_link into sk_link_src. *)
-    (* rename st_init into st_init_src. *)
-    (* rename ms into ms_src. rename m into m_src. *)
-    (* rename INIT into INITSRC. rename INITSK into INITSKSRC. rename INITMEM into INITMEMSRC. *)
-    assert(exists sk_link_src m_src, <<INITSKSRC: link_sk p_src = Some sk_link_src>>
-                                                  /\ <<LOADSRC: Sk.load_mem sk_link_src = Some m_src>>).
-    { unguard. des. inv SAFESRC. esplits; eauto. } des.
-
-    exploit sim_link_sk; eauto. i; des. fold p_tgt in LOADTGT.
-    exploit init_sim_ge_strong; eauto. i; des. clarify.
-    ss. des_ifs.
-
-    assert(SIMFPTR: SimMem.sim_val sm_init (Genv.symbol_address (Genv.globalenv sk_link_src)
-                                                                (prog_main sk_link_src) Ptrofs.zero)
-                                   (Genv.symbol_address (Genv.globalenv sk_link_tgt)
-                                                        (prog_main sk_link_tgt) Ptrofs.zero)).
-    { admit "strengthen sim_skenv specs". }
-
-    inv INITTGT. clarify.
-    exploit find_fptr_owner_bsim; eauto.
-    { unguard. des. inv SAFESRC. clarify. esplits; eauto. } i; des. clarify.
-    inv SIMMS.
-    inv MSFIND. inv FINDSRC.
-    assert(SIMRS: SimMem.sim_regset sm_init
-        (init_regs (Genv.symbol_address (Sk.load_skenv sk_link_src) (prog_main sk_link_src) Ptrofs.zero))
-        (init_regs (Genv.symbol_address (Sk.load_skenv sk_link_tgt) (prog_main sk_link_tgt) Ptrofs.zero))).
-    { u. ii. ss.
-      unfold Pregmap.set.
-      des_ifs.
-      - admit "strengthen sim_val".
-      - admit "strengthen sim_val".
-      - admit "strengthen sim_val".
-    }
-    bar.
-    exploit SIM; eauto. i; des. clear INITPROGRESS.
-    exploit INITSIM; eauto. i; des. clear INITSIM.
-
-    destruct msp; ss.
-    assert(idx = Ord.idx). { admit "easy". } clarify.
-    assert(ord = Ord.ord). { admit "easy". } clarify.
-
-    esplits; eauto.
-    - econs; eauto. econs; eauto.
-    - econs; eauto.
-      + ss. des_ifs.
-      + econs; eauto.
-      + reflexivity.
-  Qed.
-
   Theorem init_lxsim_lift_forward
           st_init_src
           (INITSRC: sem_src.(Smallstep.initial_state) st_init_src)
@@ -672,12 +597,7 @@ Section ADQINIT.
   Proof.
     inv INITSRC; ss.
     rename sk_link into sk_link_src.
-    rename st_init into st_init_src.
-    rename ms into ms_src. rename m into m_src.
-    rename INIT into INITSRC. rename INITSK into INITSKSRC. rename INITMEM into INITMEMSRC.
-    (* inv MSFIND. *)
-    (* rename blk into blk_src. rename if_sig into if_sig_src. rename FPTR into FPTRSRC. *)
-    (* rename MODSEM into MODSEMSRC. rename INTERNAL into INTERNALSRC. *)
+    rename INITSK into INITSKSRC. rename INITMEM into INITMEMSRC.
 
     exploit sim_link_sk; eauto. i; des. fold p_tgt in LOADTGT.
     exploit init_sim_ge_strong; eauto. i; des. clarify.
@@ -689,9 +609,6 @@ Section ADQINIT.
                                                         (prog_main sk_link_tgt) Ptrofs.zero)).
     { admit "strengthen sim_skenv specs". }
 
-    exploit find_fptr_owner_fsim; eauto. i; des. clarify.
-    inv SIMMS.
-    inv MSFIND. inv FINDTGT.
     assert(SIMRS: SimMem.sim_regset sm_init
         (init_regs (Genv.symbol_address (Sk.load_skenv sk_link_src) (prog_main sk_link_src) Ptrofs.zero))
         (init_regs (Genv.symbol_address (Sk.load_skenv sk_link_tgt) (prog_main sk_link_tgt) Ptrofs.zero))).
@@ -702,31 +619,40 @@ Section ADQINIT.
       - admit "strengthen sim_val".
       - admit "strengthen sim_val".
     }
-    exploit SIM; eauto. i; des.
-    bar.
-    exploit INITPROGRESS; eauto. i; des.
-    bar.
-    exploit find_fptr_owner_fsim; eauto. { econs; eauto. } i; des.
-
-    remember (ModSemPair.src msp) as srcm. revert Heqsrcm. clarify. i. clears msp.
-
-    inv SIMMS. inv FINDTGT.
-    exploit SIM; eauto. i; des.
-    exploit INITPROGRESS; eauto. i; des.
-    exploit INITSIM; eauto. i; des.
-    assert(st_init_src = st_init_src0).
-    { eapply ModSem.initial_frame_dtm; eauto. }
-    clarify.
 
     esplits; eauto.
     - econs; ss; cycle 1.
       { ii. eapply initial_state_determ; ss; eauto. }
       econs; eauto.
-      econs; eauto.
     - econs; eauto.
       + ss. des_ifs.
       + econs; eauto.
       + reflexivity.
+    (* exploit SIM; eauto. i; des. *)
+    (* bar. *)
+    (* exploit INITPROGRESS; eauto. i; des. *)
+    (* bar. *)
+    (* exploit find_fptr_owner_fsim; eauto. { econs; eauto. } i; des. *)
+
+    (* remember (ModSemPair.src msp) as srcm. revert Heqsrcm. clarify. i. clears msp. *)
+
+    (* inv SIMMS. inv FINDTGT. *)
+    (* exploit SIM; eauto. i; des. *)
+    (* exploit INITPROGRESS; eauto. i; des. *)
+    (* exploit INITSIM; eauto. i; des. *)
+    (* assert(st_init_src = st_init_src0). *)
+    (* { eapply ModSem.initial_frame_dtm; eauto. } *)
+    (* clarify. *)
+
+    (* esplits; eauto. *)
+    (* - econs; ss; cycle 1. *)
+    (*   { ii. eapply initial_state_determ; ss; eauto. } *)
+    (*   econs; eauto. *)
+    (*   econs; eauto. *)
+    (* - econs; eauto. *)
+    (*   + ss. des_ifs. *)
+    (*   + econs; eauto. *)
+    (*   + reflexivity. *)
   Qed.
 
 End ADQINIT.
@@ -765,7 +691,48 @@ Section ADQSTEP.
     generalize dependent st_tgt0.
     generalize dependent i0.
     pcofix CIH. i. pfold.
-    inv LXSIM; ss. rewrite LINKSRC in *. rewrite LINKTGT in *.
+    inv LXSIM; ss; cycle 1.
+    { (* init *)
+      des_ifs. left.
+      econs; eauto.
+      { ii. ss. inv FINALSRC. }
+      econs; eauto; cycle 1.
+      { eapply callstate_receptive_at. }
+      ii. ss. des_ifs.
+      inv STEPSRC.
+      exploit find_fptr_owner_fsim; eauto. i; des. clarify.
+      inv MSFIND. inv FINDTGT.
+      inv SIMMS.
+
+
+      specialize (SIM sm0).
+      exploit SIM; eauto. i; des.
+
+      (* specialize (SIM (SimMem.lift sm0)). *)
+      (* exploit SIM; eauto. *)
+      (* { eapply SimMem.lift_sim_val; eauto. } *)
+      (* { ii. eapply SimMem.lift_sim_val; eauto. } *)
+      (* { eapply SimMem.lift_wf; eauto. } *)
+      (* { u. eapply SimSymb.mlift_preserves_sim_skenv; eauto. } *)
+      (* { ss. erewrite SimMem.lift_src. eauto. } *)
+      (* i; des. *)
+
+
+      esplits; eauto.
+      - left. eapply plus_one.
+        econs; eauto; cycle 1.
+        + econs; eauto.
+          * ss. des_ifs. econs; eauto; ss.
+          (* * erewrite SimMem.lift_tgt in INITTGT. eauto. *)
+        + eapply callstate_determinate_at; eauto.
+      - instantiate (1:= idx_init).
+        right. eapply CIH.
+        instantiate (1:= sm_init).
+        econs 1; try apply SIM0; eauto.
+        + ss. des_ifs. eapply mle_preserves_sim_ge; eauto.
+        + eapply lxsim_stack_le; eauto.
+    }
+    rewrite LINKSRC in *. rewrite LINKTGT in *.
     punfold TOP. inv TOP.
 
 
@@ -782,7 +749,7 @@ Section ADQSTEP.
           { exfalso. eauto. }
           { exfalso. eapply SAFESRC0. u. eauto. }
           exploit STEP; eauto. i; des_safe.
-          exists i1, ((Frame.mk ms_tgt rs_init_tgt st_tgt1) :: tail_tgt).
+          exists i1, (State ((Frame.mk ms_tgt rs_init_tgt st_tgt1) :: tail_tgt)).
           esplits; eauto.
           { des.
             - left. eapply lift_dplus; eauto.
@@ -805,7 +772,7 @@ Section ADQSTEP.
         * econs 1; eauto.
           ii. inv STEPTGT; ModSem.tac.
           ss. exploit STEP; eauto. i; des_safe.
-          exists i1, ((Frame.mk ms_src rs_init_src st_src1) :: tail_src).
+          exists i1, (State ((Frame.mk ms_src rs_init_src st_src1) :: tail_src)).
           esplits; eauto.
           { des.
             - left. eapply lift_plus; eauto.
@@ -832,9 +799,7 @@ Section ADQSTEP.
         { inv SAFESRC0. ss. exfalso. eapply ModSem.call_return_disjoint; eauto. u. esplits; eauto. }
         ss; des_ifs.
         inv SAFESRC0; ss; ModSem.tac.
-        esplits; eauto. econs; ss; eauto.
-        - admit "find fptr owner progress".
-        - admit "initial_frame progress". }
+        esplits; eauto. econs; ss; eauto. }
 
       (* ii. unfold safe in *. ss. specialize (SAFESRC _ (star_refl _ _ _)). des. *)
       (* { admit "final forward". } *)
@@ -853,40 +818,27 @@ Section ADQSTEP.
       eapply mle_preserves_sim_ge with (sm2:= sm_arg) in GE; eauto.
       (* Note: Coq bug STILL not fixed!!! there is no name like sm2. *)
 
-      exploit find_fptr_owner_bsim; eauto.
-      { esplits; eauto. admit "use SAFESRC". }
-      i; des.
-
-      inv SIMMS.
-      dup FINDSRC. dup MSFIND.
-      inv FINDSRC0; ss. inv MSFIND0; ss.
-      specialize (SIM (SimMem.lift sm_arg)).
-      exploit SIM; eauto.
-      { eapply SimMem.lift_sim_val; eauto. }
-      (* { instantiate (2:= PC). rewrite FPTR; ss. des_ifs. unfold Genv.find_funct_ptr. des_ifs. } *)
-      (* { rewrite FPTR0. ss. des_ifs. unfold Genv.find_funct_ptr. des_ifs. } *)
-      { ii. eapply SimMem.lift_sim_val; eauto. }
-      { eapply SimMem.lift_wf; eauto. }
-      { u. eapply SimSymb.mlift_preserves_sim_skenv; eauto. }
-      i; des_safe.
-      exploit INITSIM; eauto. { rewrite SimMem.lift_tgt. eauto. } i; des_safe.
+      clarify.
       esplits; eauto.
-      + left. apply plus_one. econs; ss; eauto. { erewrite <- SimMem.lift_src. eauto. }
+      + left. apply plus_one. econs; ss; eauto.
       + right. eapply CIH; eauto.
         {
           instantiate (1:= (SimMem.lift sm_arg)).
-          econs.
+          erewrite <- SimMem.lift_src. erewrite <- SimMem.lift_tgt.
+          econs 2; eauto.
           * ss. des_ifs. eapply mlift_preserves_sim_ge; eauto.
           * instantiate (1:= (SimMem.lift sm_arg)).
             econs; [eassumption|..]; revgoals.
             { ii. exploit K; eauto. i; des_safe. esplits; eauto.
               ii. exploit KSTEP; eauto. i; des_safe. pclearbot. esplits; eauto.
             }
+            { reflexivity. }
             { etransitivity; eauto. }
             { ss. des_ifs. }
             { eauto. }
           * reflexivity.
-          * eauto.
+          * eapply SimMem.lift_wf; eauto.
+          * ii. eapply SimMem.lift_sim_val; eauto. 
         }
 
 
@@ -922,10 +874,13 @@ Section ADQSTEP.
         move AFTER at bottom.
         move STACK at bottom.
         inv STACK. ss.
-        exploit K; try apply RSREL0; eauto. { erewrite <- mcompat_src; eauto. } i; des.
+        exploit K; try apply RSREL; eauto.
+        { etransitivity; eauto. }
+        { erewrite <- mcompat_src in *; eauto. }
+        i; des.
         esplits; eauto.
-        econs 3; ss; eauto.
-        erewrite mcompat_tgt; eauto.
+        econs 4; ss; eauto.
+        erewrite <- mcompat_tgt in *; eauto.
       }
       i.
       econs 1; eauto. ss. des_ifs.
@@ -937,28 +892,31 @@ Section ADQSTEP.
       { eapply FINAL. }
       i; des. clarify. clear_tac.
       inv STACK. ss.
-      exploit K; eauto.
+      exploit K; try apply RSREL; eauto.
+      { etransitivity; eauto. }
       { specialize (SAFESRC _ (star_refl _ _ _)).
         des; ss.
         { inv SAFESRC. }
         inv SAFESRC; ModSem.tac. ss.
-        determ_tac ModSem.final_frame_dtm. erewrite <- mcompat_src; eauto.
+        determ_tac ModSem.final_frame_dtm. erewrite <- mcompat_src in *; eauto.
       }
       i; des. exploit KSTEP; eauto. i; des.
       esplits; eauto.
       + left. apply plus_one.
-        econs 3; ss; eauto.
-        erewrite mcompat_src; eauto.
+        econs 4; ss; eauto.
+        erewrite <- mcompat_src in *; eauto.
       + right. eapply CIH; eauto.
         instantiate (1:= (SimMem.unlift sm_arg sm0)).
         econs; ss; cycle 1.
         { eauto. }
         { etransitivity; eauto.
-          eapply SimMem.unlift_spec; eauto. }
+          eapply SimMem.unlift_spec; eauto.
+          etransitivity; eauto. }
         { erewrite mcompat_tgt in AFTER; eauto. determ_tac ModSem.after_external_dtm. eauto. }
         { des_ifs.
           eapply mle_preserves_sim_ge; eauto.
-          eapply SimMem.unlift_spec; eauto. }
+          eapply SimMem.unlift_spec; eauto.
+          etransitivity; eauto. }
   Unshelve.
     all: ss.
   Qed.
@@ -968,7 +926,7 @@ End ADQSTEP.
 
 
 
-Section ADEQUACY.
+Section ADQ.
 
   Context `{SM: SimMem.class}.
   Context {SS: SimSymb.class SM}.
@@ -989,248 +947,24 @@ Section ADEQUACY.
     econstructor 1 with (order := ord); eauto.
     econs; eauto.
     { eapply wf_ord; eauto. }
-    econs 2; ss; eauto.
-    -
-  Qed.
-
-  Theorem adequacy_local
-          sem_src
-          (LOADSRC: load p_src = Some sem_src)
-    :
-      exists sem_tgt, <<LOADTGT: load p_tgt = Some sem_tgt>> /\ <<SIM: mixed_simulation sem_src sem_tgt>>
-  .
-  Proof.
-    (* exploit sim_load; eauto. i; des. *)
-    subst_locals. unfold load in *. des_ifs_safe.
-    exploit sim_link_sk; eauto. i; des. des_ifs_safe. clarify.
-    rename t into sk_src. rename sk_link_tgt into sk_tgt.
-    esplits; eauto.
-
-
-    exploit sim_progpair_sim_loadpair; eauto. i; des.
-    assert(LPSIM := SIM).
-    inv SIM.
-    econs; eauto.
-    econs; eauto.
-
-    eapply xsim_init_forward; ss.
-    ii. inv INITSRC. clarify.
-    exploit SimSymb.sim_sk_load_sim_skenv; eauto. i; des. clarify.
-    exploit find_fptr_owner_bsim; eauto.
-    { instantiate (2:= (Genv.symbol_address (Sk.load_skenv sk_src) (prog_main sk_src) Integers.Ptrofs.zero)).
-      instantiate (1:= (Genv.symbol_address (Sk.load_skenv sk_tgt) (prog_main sk_tgt) Integers.Ptrofs.zero)).
-      admit "main ptr should be related. obligate this to sim_skenv". }
-    { admit "???". }
-    { unfold LoadPair.ge_src. unfold load_genv, load_modsems in MSFIND.
-      admit "???".
+    destruct (classic (pp <> [])); cycle 1.
+    { apply NNPP in H. clarify.
+      ss.
+      econs; eauto.
+      ii. ss. inv INITSRC. ss.
     }
-    i; des.
-
-    esplits; eauto.
-    - econs; ss; eauto.
-      + admit "".
-      + admit "determinacy".
-    -
-
+    rename H into NOTNIL.
+    econs 1; ss; eauto.
     ii.
-    inv ujjj
-    eapply xsim_init_backward; ss.
-    {
-      ii. inv INITSRC. clarify.
-      exploit SimSymb.sim_sk_load_sim_skenv; eauto. i; des. clarify.
-      exploit find_fptr_owner_bsim; eauto.
-      { instantiate (2:= (Genv.symbol_address (Sk.load_skenv sk_src) (prog_main sk_src) Integers.Ptrofs.zero)).
-        instantiate (1:= (Genv.symbol_address (Sk.load_skenv sk_tgt) (prog_main sk_tgt) Integers.Ptrofs.zero)).
-        admit "main ptr should be related. obligate this to sim_skenv". }
-      { }
-      esplits; eauto. econs; ss; eauto.
-      -
-      admit "progress".
-    }
-
-
-    exploit sim_progpair_sim_gepair; eauto. i; des. ss.
-    esplits; eauto. clarify.
-    inv SIM; ss.
-    econstructor 1 with (order := gep.(GePair.ord)); eauto.
-    econs; eauto.
-    eapply xsim_init_backward; ss.
-    { (* progress *)
-      i. inv INITSRC. ss.
-      inv MSFIND. ss.
-      unfold Genv.symbol_address in *. des_ifs.
-      Print SimSymb.sim_sk_weak.
-      apply SimSymb.sim_sk_sim_sk_weak in SIMSK.
-      admit "sim_skenv should have some info################!!!!!!!!!!!!!!!!!!!!".
-    }
-    { (* init *)
-      i. inv INITTGT.
-      rename ms into ms_tgt.
-      assert(exists ms_src, <<SIMMS: sim_modsem order ms_src ms_tgt>>).
-      { admit "". } i; des.
-      inv SIMMS.
-      inv MSFIND.
-      unfold Genv.symbol_address in *. des_ifs.
-      rename Heq0 into MAINTGT. rename blk into blk_tgt. rename m into m_tgt. rename INITMEM into MEMTGT.
-      (* assert(exists blk_tgt m_tgt sm0, *)
-      (*           <<WF: SimMem.wf sm0>> *)
-      (*           /\ <<MEMTGT: sk_tgt.(Sk.load_mem) = Some m_tgt>> *)
-      (*           /\ <<MAINTGT: Genv.find_symbol (Sk.load_skenv sk_src) (prog_main sk_src) = Some blk_tgt>> *)
-      (*           /\ <<SIMFPTR: SimMem.sim_block sm0 blk_src blk_tgt>> *)
-      (*           /\ <<MCOMPAT: sm0.(SimMem.src_mem) = m_src /\ sm0.(SimMem.tgt_mem) = m_tgt>>). *)
-      assert(exists blk_src m_src sm0,
-                <<WF: SimMem.wf sm0>>
-                /\ <<MEMSRC: sk_src.(Sk.load_mem) = Some m_src>>
-                /\ <<MAINSRC: Genv.find_symbol (Sk.load_skenv sk_src) (prog_main sk_src) = Some blk_src>>
-                /\ <<SIMFPTR: SimMem.sim_block sm0 blk_src blk_tgt>>
-                /\ <<MCOMPAT: sm0.(SimMem.src_mem) = m_src /\ sm0.(SimMem.tgt_mem) = m_tgt>>).
-      { admit "sim_skenv should have some info################!!!!!!!!!!!!!!!!!!!!". }
-      i; des.
-
-      hexploit SIM; eauto.
-      { instantiate (1:= None). instantiate (1:= None). econs 2; eauto. }
-      { instantiate (1:= (Asmregs.Pregmap.init Vundef)). instantiate (1:= (Asmregs.Pregmap.init Vundef)).
-        admit "undef sim_val".
-      }
-      i; des.
-      exploit STEP; eauto.
-      { rewrite MCOMPAT0. eauto. }
-      i; des.
-      esplits; eauto.
-      esplits; eauto.
-      rename m into m_tgt.
-      rename st_init into st_init_tgt.
-      rename ms into ms_tgt.
-      rename INITSK into INITSKTGT.
-      rename INITMEM into INITMEMTGT.
-      inv MSFIND. ss. clarify.
-      rename MODSEM into MODSEMTGT.
-      rename 
-    }
-    { (* init *)
-      i. inv INITSRC. inv MSFIND. ss. clarify.
-      unfold Genv.symbol_address in *. des_ifs.
-      rename Heq into MAINSRC. rename blk into blk_src. rename m into m_src. rename INITMEM into MEMSRC.
-      assert(exists blk_tgt m_tgt sm0,
-                <<MEMTGT: sk_tgt.(Sk.load_mem) = Some m_tgt>>
-                /\ <<MAINTGT: Genv.find_symbol (Sk.load_skenv sk_src) (prog_main sk_src) = Some blk_tgt>>
-                /\ <<SIMFPTR: SimMem.sim_block sm0 blk_src blk_tgt>>
-                /\ <<SIMMS: sm0.(SimMem.src_mem) = m_src /\ sm0.(SimMem.tgt_mem) = m_tgt>>).
-      { admit "sim_skenv should have some info################!!!!!!!!!!!!!!!!!!!!". }
-      des.
-      esplits; eauto.
-    }
-    i. ss.
-    tttttttttttttttttttttttt
-    exploit sim_load; eauto. i; des.
-    esplits; eauto.
-
-    unfold sem in *. des_ifs. rename t into init_sk_tgt. rename t0 into init_sk_src.
-    inv SIMPROG.
-    inv SIMMOD. admit "".
-    assert(Forall2 sim_modsem
-    assert(exists wfo, 
-    econs; eauto.
-    econs; eauto.
-    (* Each modsem has mixed sim *)
-
-    assert(Forall3 sim_modsem p_src p_tgt).
-    eapply Forall3_impl with (Q:= const sim_modsem) in SIMMOD.
-    
+    exploit init_lxsim_lift_forward; eauto. i; des.
+    ss.
+    assert(exists sk_link_src, link_sk (ProgPair.src pp) = Some sk_link_src).
+    { inv INITSRC. eauto. }
+    assert(exists sk_link_tgt, link_sk (ProgPair.tgt pp) = Some sk_link_tgt).
+    { inv INITTGT. inv INIT. eauto. }
+    des.
+    hexploit lxsim_lift_xsim; eauto.
   Qed.
 
+End ADQ.
 
-End ADEQUACY.
-
-
-Context `{Linker symbinj}.
-Context `{SM: SimMem}.
-
-(* Inductive sim_mod `{SM: SimMem} (si: symbinj) (m_src m_tgt: Mod.t): Prop := *)
-(* | sim_mod_intro *)
-(*     (SIMSK: sim_sk si m_src.(Mod.sk) m_tgt.(Mod.sk)) *)
-(* . *)
-
-Axiom sim_skenv: list symbinj -> SkEnv.t -> SkEnv.t -> Prop.
-Axiom sim_modsem: symbinj -> ModSem.t -> ModSem.t -> Prop.
-
-
-
-Inductive sim_prog (p_src p_tgt: program): Prop :=
-| sim_prog_intro
-    sis
-    (SIMMOD: Forall3 sim_mod sis p_src p_tgt)
-    si_prog
-    (LINKSI: link_list sis = Some si_prog)
-    (SIMMS: forall
-        skenv_src skenv_tgt
-        (SIMSKENV: sim_skenv sis skenv_src skenv_tgt)
-      ,
-        Forall2 (fun m_src m_tgt => sim_modsem (m_src.(Mod.get_modsem) skenv_src m_src.(Mod.data))
-                                               (m_tgt.(Mod.get_modsem) skenv_tgt m_tgt.(Mod.data))) p_src p_tgt)
-.
-
-Section TRANSF.
-
-  Variable p: program.
-
-End TRANSF.
-
-Section ADEQUACY.
-
-  Variable p_src p_tgt: program.
-  Hypothesis SIMPROG: sim_prog p_src p_tgt.
-
-    Theorem xsim_properties_embedded
-            L1 L2
-            (EMBEDDED: embedded ord0 ord1)
-            (XSIM: xsim_properties L1 L2 idx0 ord0)
-      :
-        <<XSIM: xsim_properties L1 L2 idx1 ord1>>
-    .
-    Proof.
-      admit "easy".
-    Qed.
-
-  End LINK_WFO.
-
-  Lemma sim_load
-        sem_src
-        (LOADSRC: sem p_src = Some sem_src)
-    :
-      exists sem_tgt, <<LOADTGT: sem p_tgt = Some sem_tgt>>
-  .
-  Proof.
-    unfold sem in *.
-    des_ifs.
-    { esplits; eauto. }
-    exfalso.
-    unfold init_sk in *.
-    admit "".
-  Qed.
-
-  Theorem adequacy_machine
-          sem_src
-          (LOADSRC: sem p_src = Some sem_src)
-    :
-      exists sem_tgt, <<LOADTGT: sem p_tgt = Some sem_tgt>> /\ <<SIM: mixed_simulation sem_src sem_tgt>>
-  .
-  Proof.
-    exploit sim_load; eauto. i; des.
-    esplits; eauto.
-
-    unfold sem in *. des_ifs. rename t into init_sk_tgt. rename t0 into init_sk_src.
-    inv SIMPROG.
-    inv SIMMOD. admit "".
-    assert(Forall2 sim_modsem
-    assert(exists wfo, 
-    econs; eauto.
-    econs; eauto.
-    (* Each modsem has mixed sim *)
-
-    assert(Forall3 sim_modsem p_src p_tgt).
-    eapply Forall3_impl with (Q:= const sim_modsem) in SIMMOD.
-    
-  Qed.
-
-End ADEQUACY.
